Garden/Halo2/proof.v
@@ -14,6 +14,23 @@ Module Assignment.
   Arguments t : clear implicits.
 End Assignment.
 
+Module Evaluation.
+  Record t {columns : Columns.t} : Set := {
+    assignment : Assignment.t columns;
+    row : Z;
+    nb_rows : Z;
+  }.
+  Arguments t : clear implicits.
+
+  Class C {columns : Columns.t} {p : Z} `{Prime p}
+      (A B : Type) : Type := {
+    eval : t columns -> A -> B;
+  }.
+End Evaluation.
+
+Notation "⟦ x ⟧ ρ" := (Evaluation.eval ρ x)
+  (at level 10, x at level 200, ρ at level 9).
+
 Definition rotated_row
     (row nb_rows : Z)
     (rotation : Rotation.t)
@@ -27,10 +44,11 @@ Section Semantics.
 
   Definition eval_selector
       (assignment : Assignment.t columns)
-      (row : Z)
+      (row nb_rows : Z)
       (selector : columns.(Columns.Selector))
       : Z :=
-    UnOp.from (assignment.(Assignment.selector) selector row).
+    UnOp.from
+      (assignment.(Assignment.selector) selector (row mod nb_rows)).
 
   Fixpoint eval_expression
       (assignment : Assignment.t columns)
@@ -41,7 +59,7 @@ Section Semantics.
     | Expression.Constant value =>
         UnOp.from value
     | Expression.Selector selector =>
-        eval_selector assignment row selector
+        eval_selector assignment row nb_rows selector
     | Expression.Fixed fixed rotation =>
         UnOp.from
           (assignment.(Assignment.fixed)
@@ -84,7 +102,7 @@ Section Semantics.
       : Prop :=
     match constraint with
     | Constraint.Select selector constraint =>
-        eval_selector assignment row selector <> 0 ->
+        eval_selector assignment row nb_rows selector <> 0 ->
           eval_constraint assignment row nb_rows constraint
     | Constraint.Equal lhs rhs =>
         eval_expression assignment row nb_rows lhs =
@@ -92,6 +110,7 @@ Section Semantics.
     | Constraint.EqualZeroToPrecise expression =>
         eval_expression assignment row nb_rows expression = 0
     end.
+  Arguments eval_constraint _ _ _ _ /.
 
   Definition eval_named_constraint
       (assignment : Assignment.t columns)
@@ -100,13 +119,22 @@ Section Semantics.
       : Prop :=
     let '(_, constraint) := constraint in
     eval_constraint assignment row nb_rows constraint.
+  Arguments eval_named_constraint _ _ _ _ /.
 
-  Definition eval_constraints
+  Fixpoint eval_constraints
       (assignment : Assignment.t columns)
       (row nb_rows : Z)
       (constraints : Constraints.t columns)
       : Prop :=
-    List.Forall (eval_named_constraint assignment row nb_rows) constraints.
+    match constraints with
+    | [] => True
+    | [constraint] =>
+        eval_named_constraint assignment row nb_rows constraint
+    | constraint :: constraints =>
+        eval_named_constraint assignment row nb_rows constraint /\
+        eval_constraints assignment row nb_rows constraints
+    end.
+  Arguments eval_constraints _ _ _ _ /.
 
   Definition eval_gate
       (assignment : Assignment.t columns)
@@ -118,13 +146,22 @@ Section Semantics.
       row
       nb_rows
       gate.(Gate.constraints).
+  Arguments eval_gate _ _ _ _ /.
 
-  Definition eval_gates
+  Fixpoint eval_gates
       (assignment : Assignment.t columns)
       (row nb_rows : Z)
       (gates : list (Gate.t columns))
       : Prop :=
-    List.Forall (eval_gate assignment row nb_rows) gates.
+    match gates with
+    | [] => True
+    | [gate] =>
+        eval_gate assignment row nb_rows gate
+    | gate :: gates =>
+        eval_gate assignment row nb_rows gate /\
+        eval_gates assignment row nb_rows gates
+    end.
+  Arguments eval_gates _ _ _ _ /.
 
   Definition eval_constraint_system_gates
       (assignment : Assignment.t columns)
@@ -138,5 +175,75 @@ Section Semantics.
         row
         nb_rows
         system.(ConstraintSystem.gates).
+
+  Global Instance SelectorIsEvaluable :
+      Evaluation.C columns.(Columns.Selector) Z := {
+    Evaluation.eval ρ selector :=
+      eval_selector
+        ρ.(Evaluation.assignment)
+        ρ.(Evaluation.row)
+        ρ.(Evaluation.nb_rows)
+        selector;
+  }.
+
+  Global Instance ExpressionIsEvaluable :
+      Evaluation.C (Expression.t columns) Z := {
+    Evaluation.eval ρ expression :=
+      eval_expression
+        ρ.(Evaluation.assignment)
+        ρ.(Evaluation.row)
+        ρ.(Evaluation.nb_rows)
+        expression;
+  }.
+
+  Global Instance ConstraintIsEvaluable :
+      Evaluation.C (Constraint.t columns) Prop := {
+    Evaluation.eval ρ constraint :=
+      eval_constraint
+        ρ.(Evaluation.assignment)
+        ρ.(Evaluation.row)
+        ρ.(Evaluation.nb_rows)
+        constraint;
+  }.
+
+  Global Instance NamedConstraintIsEvaluable :
+      Evaluation.C (option string * Constraint.t columns) Prop := {
+    Evaluation.eval ρ constraint :=
+      eval_named_constraint
+        ρ.(Evaluation.assignment)
+        ρ.(Evaluation.row)
+        ρ.(Evaluation.nb_rows)
+        constraint;
+  }.
+
+  Global Instance ConstraintsIsEvaluable :
+      Evaluation.C (Constraints.t columns) Prop := {
+    Evaluation.eval ρ constraints :=
+      eval_constraints
+        ρ.(Evaluation.assignment)
+        ρ.(Evaluation.row)
+        ρ.(Evaluation.nb_rows)
+        constraints;
+  }.
+
+  Global Instance GateIsEvaluable :
+      Evaluation.C (Gate.t columns) Prop := {
+    Evaluation.eval ρ gate :=
+      eval_gate
+        ρ.(Evaluation.assignment)
+        ρ.(Evaluation.row)
+        ρ.(Evaluation.nb_rows)
+        gate;
+  }.
+
+  Global Instance GatesIsEvaluable :
+      Evaluation.C (list (Gate.t columns)) Prop := {
+    Evaluation.eval ρ gates :=
+      eval_gates
+        ρ.(Evaluation.assignment)
+        ρ.(Evaluation.row)
+        ρ.(Evaluation.nb_rows)
+        gates;
+  }.
 
 End Semantics.
